

## Lista de exercícios

1.  $A = \begin{bmatrix} x & 1 \\ 5 & 2 \end{bmatrix}$  é inversa de  $B = \begin{bmatrix} 3 & -1 \\ y & 2 \end{bmatrix}$

$$\begin{bmatrix} x & 1 \\ 5 & 2 \end{bmatrix} \cdot \begin{bmatrix} 3 & -1 \\ y & 2 \end{bmatrix} = \begin{bmatrix} 1 & 0 \\ 0 & 1 \end{bmatrix}$$

$$\begin{bmatrix} 3x + y & -x + 2 \\ 15 + 3y & -5 + 6 \end{bmatrix}$$

$$\begin{cases} 3x + y = 1 & -x + 2 = 0 \rightarrow x = 2 \\ 15 + 3y = 0 & -5 + 6 = 1 \end{cases}$$

$$3x + y = 1$$

$$x + y = ?$$

$$3 \cdot 2 + y = 1$$

$$2 + (-5) = 2 - 5 = -3 //$$

$$6 + y = 1$$

alternativa: (c) //

$$y = -5$$

2

$$A = \begin{vmatrix} 1 & 0 & 1 \\ k & 1 & 3 \\ 1 & k & 3 \end{vmatrix} \quad \begin{vmatrix} 1 & 3k & 0 \\ 1 & 0 \\ 3 & 0 & k^2 \end{vmatrix}$$

pl não admitir a inversão

$$\det A = 0$$

$$= k^2 + 3 - 1 - 3k$$

$$= k^2 + 2 - 3k$$

$$\Delta = (-3)^2 - 4 \cdot 1 \cdot 2$$

$$\Delta = 9 - 8$$

$$\Delta = 1$$

$$k = \frac{-(-3) \pm \sqrt{1}}{2 \cdot 1}$$

$$k' = \frac{4}{2} = 2 //$$

$$k'' = \frac{2}{2} = 1 //$$

alternativa (C) //

3

$$A = \begin{vmatrix} 3 & 5 \\ 2 & 4 \end{vmatrix}$$

$$\Rightarrow \det A = 12 - 10 = 2$$

$$B = A^{-1} = \begin{vmatrix} 4 & -5 \\ -2 & 3 \end{vmatrix} \div 2$$

$$B = \begin{vmatrix} 2 & -5/2 \\ -1 & 3/2 \end{vmatrix} //$$

alternativa (C) //

4

$$\begin{vmatrix} x & 1 & 2 \\ 3 & 1 & 2 \\ 10 & 1 & x \end{vmatrix} \quad \begin{vmatrix} x & x^2 \\ 2x & x \\ 3x & 3 \end{vmatrix}$$

$$\Rightarrow x^2 + 26 - 20 - 5x \Rightarrow x^2 - 5x + 6 \neq 0$$

$$x = \frac{-(-5) \pm \sqrt{1}}{2 \cdot 1}$$

$$x = \frac{5 \pm 1}{2}$$

$$x' = \frac{6}{2} = 3$$

$$x'' = \frac{4}{2} = 2$$

$$x \neq 3 //$$

$$x \neq 2 //$$

$$\Delta = (-5)^2 - 4 \cdot 1 \cdot 6$$

$$\Delta = 25 - 24$$

$$\Delta = 1$$

$$\{x \neq 3 \text{ e } x \neq 2\} //$$

tilibra



5.  $A = \begin{bmatrix} -1 & -1 & 2 \\ 2 & 1 & -2 \\ 1 & 1 & -1 \end{bmatrix}$

$$2 + 2 + 2 = 6$$

$$\det A = \begin{vmatrix} -1 & -1 & 2 \\ 2 & 1 & -2 \\ 1 & 1 & -1 \end{vmatrix} = \begin{vmatrix} -1 & -1 \\ 2 & 1 \end{vmatrix} - 2 \begin{vmatrix} -1 & 2 \\ 1 & -1 \end{vmatrix} = 1 - 6 = -5$$

$$1 + 2 + 4 = 7$$

$$A' = \begin{bmatrix} 1 & 0 & 1 \\ 1 & -1 & 0 \\ 0 & 2 & 1 \end{bmatrix}$$

$$\bar{A} = (A')^T = \begin{bmatrix} 1 & 1 & 0 \\ 0 & -1 & 2 \\ 1 & 0 & 1 \end{bmatrix} \div 1$$

$$A = \begin{bmatrix} -1 & -1 & 2 \\ 2 & 1 & -2 \\ 1 & 1 & -1 \end{bmatrix}$$

$$A^{-1} = \begin{bmatrix} 1 & 1 & 0 \\ 0 & -1 & 2 \\ 1 & 0 & 1 \end{bmatrix}$$

$$A + A^{-1} = \begin{bmatrix} 0 & 0 & 2 \\ 2 & 0 & 0 \\ 2 & 1 & 0 \end{bmatrix} //$$

alternativa (b) //

A

$$6 \quad ((XA)^t)^t = B^t$$

$$XAA^{-1} = B^t A^{-1}$$

$$X = B^t A^{-1}$$

alternativa (B)

$$7. \quad A \cdot B = C$$

$$A = C/B$$

$$C = \begin{bmatrix} 4x+5y \\ 5x+6y \end{bmatrix}$$

$$B = \begin{bmatrix} x \\ y \end{bmatrix}$$

$$\begin{bmatrix} 4x/x + 5y/y \\ 5x/x + 6y/y \end{bmatrix} \Rightarrow A = \begin{bmatrix} 4 & 5 \\ 5 & 6 \end{bmatrix}$$

$$A^{-1} = \begin{bmatrix} -4 & 5 \\ 5 & -6 \end{bmatrix}$$

alternativa (D)

9. a)  $(A+B) \cdot (A-B)$

$$A^2 - AB + BA - B^2 //$$

b)  $(A+B)^2 = A^2 + 2 \cdot A \cdot B + B^2$

$$(A+B)^2 = (A+B) \cdot (A+B) = A^2 + AB + BA + B^2$$

$$A^2 + AB + BA + B^2 = A^2 + 2AB + B^2$$

$$AB = BA //$$

c)  $\det(-A) = (-1)^n \cdot \det A = \det A \neq 0$

d)  $\det(AB) = 1$

$$\det(A) \cdot \det(B) = 1$$

$$\det B = 1$$

$$\frac{\det(A)}{\det(-A)} = \frac{\det(A)}{\det(A)} = 1 //$$

$$\det A //$$

$$\det(-A) \quad \det(A)$$